src/State.v
@@ -1,40 +1,138 @@
 
+From Coq Require Import ZArith.
 From mathcomp Require Import ssreflect ssrbool eqtype seq.
 From nbits Require Import NBits.
-From ssrlib Require Import Types SsrOrdered Store.
-From BitBlasting Require Import Var Typ TypEnv.
+From ssrlib Require Import Var Types SsrOrder Store ZAriths FMaps.
+From BitBlasting Require Import Typ TypEnv.
 
 Set Implicit Arguments.
 Unset Strict Implicit.
 Import Prenex Implicits.
 
-Module ValueType <: HasDefaultTyp.
-  Definition t := bits.
+Module BitsValueType <: HasDefaultTyp.
+  Definition t : Type := bits.
   Definition default : t := [::].
-End ValueType.
+End BitsValueType.
 
-Module Store := RealizableTStoreAdapter VarOrder ValueType.
+Module ZValueType <: HasDefaultTyp.
+  Definition t : Type := Z.
+  Definition default : t := 0%Z.
+End ZValueType.
 
-Inductive state : Type :=
-| OK of Store.t
-| ERR.
+Module Type BitsStore (V : SsrOrder) (TE : TypEnv with Module SE := V).
 
+  Local Notation var := V.t.
+  Local Notation value := bits.
 
+  Parameter t : Type.
+  Parameter acc : var -> t -> value.
+  Parameter upd : var -> value -> t -> t.
+  Parameter upd2 : var -> value -> var -> value -> t -> t.
+  Parameter acc_upd_eq : forall {x y v s}, x == y -> acc x (upd y v s) = v.
+  Parameter acc_upd_neq : forall {x y v s}, x != y -> acc x (upd y v s) = acc x s.
+  Parameter acc_upd2_eq1 :
+    forall {x y1 v1 y2 v2 s},
+      x == y1 -> x != y2 -> acc x (upd2 y1 v1 y2 v2 s) = v1.
+  Parameter acc_upd2_eq2 :
+    forall {x y1 v1 y2 v2 s},
+      x == y2 -> acc x (upd2 y1 v1 y2 v2 s) = v2.
+  Parameter acc_upd2_neq :
+    forall {x y1 v1 y2 v2 s},
+      x != y1 -> x != y2 -> acc x (upd2 y1 v1 y2 v2 s) = acc x s.
+  Parameter Upd : var -> value -> t -> t -> Prop.
+  Definition Upd2 x1 v1 x2 v2 (s1 s2 : t) : Prop :=
+    forall y, acc y s2 = acc y (upd x2 v2 (upd x1 v1 s1)).
+  Parameter Equal : t -> t -> Prop.
+  Parameter Upd_upd : forall x v s, Upd x v s (upd x v s).
+  Parameter Upd2_upd :
+    forall x1 v1 x2 v2 s, Upd2 x1 v1 x2 v2 s (upd x2 v2 (upd x1 v1 s)).
+  Parameter Upd2_upd2 : forall x1 v1 x2 v2 s, Upd2 x1 v1 x2 v2 s (upd2 x1 v1 x2 v2 s).
+  Parameter acc_Upd_eq : forall x y v s1 s2, x == y -> Upd y v s1 s2 -> acc x s2 = v.
+  Parameter acc_Upd_neq :
+    forall x y v s1 s2, x != y -> Upd y v s1 s2 -> acc x s2 = acc x s1.
+  Parameter acc_Upd2_eq1 :
+    forall x y1 v1 y2 v2 s1 s2,
+      x == y1 -> x != y2 -> Upd2 y1 v1 y2 v2 s1 s2 -> acc x s2 = v1.
+  Parameter acc_Upd2_eq2 :
+    forall x y1 v1 y2 v2 s1 s2, x == y2 -> Upd2 y1 v1 y2 v2 s1 s2 -> acc x s2 = v2.
+  Parameter acc_Upd2_neq :
+    forall x y1 v1 y2 v2 s1 s2,
+      x != y1 -> x != y2 -> Upd2 y1 v1 y2 v2 s1 s2 -> acc x s2 = acc x s1.
+  Parameter Equal_refl : forall s, Equal s s.
+  Parameter Equal_sym : forall s1 s2, Equal s1 s2 -> Equal s2 s1.
+  Parameter Equal_trans : forall s1 s2 s3, Equal s1 s2 -> Equal s2 s3 -> Equal s1 s3.
+  Parameter Equal_ST : RelationClasses.Equivalence Equal.
+  Parameter Equal_upd_Equal :
+    forall v e s1 s2, Equal s1 s2 -> Equal (upd v e s1) (upd v e s2).
+  Parameter Equal_Upd_Equal :
+    forall v e s1 s2 s3 s4,
+      Upd v e s1 s2 -> Upd v e s3 s4 -> Equal s1 s3 -> Equal s2 s4.
+  Parameter Upd_pred_Equal :
+    forall v e s1 s2 s, Upd v e s1 s2 -> Equal s1 s -> Upd v e s s2.
+  Parameter Upd_succ_Equal :
+    forall v e s1 s2 s, Upd v e s1 s2 -> Equal s2 s -> Upd v e s1 s.
 
-(* A store conforms to a typing environment if for every variable in the typing
-   environment, the size of its type in the typing environment is the same as
-   the size of its value in the store *)
+  Parameter conform : t -> TE.env -> Prop.
+  Parameter conform_mem :
+    forall v s te, conform s te -> TE.mem v te -> TE.vsize v te = size (acc v s).
+  Parameter conform_upd :
+    forall x ty v s te,
+      sizeof_typ ty = size v -> conform s te -> conform (upd x v s) (TE.add x ty te).
 
-Definition conform (s : Store.t) (te : TypEnv.t) : Prop :=
-  forall (v : var),
-    TypEnv.mem v te -> TypEnv.vsize v te = size (Store.acc v s).
+End BitsStore.
 
-Lemma conform_upd x ty v s te :
-  sizeof_typ ty = size v ->
-  conform s te -> conform (Store.upd x v s) (TypEnv.add x ty te).
-Proof.
-  move=> Hs Hcon y. case Hyx: (y == x).
-  - by rewrite (TypEnv.vsize_add_eq Hyx) (Store.acc_upd_eq Hyx).
-  - move/idP/negP: Hyx => Hyx. rewrite (TypEnv.mem_add_neq Hyx) => Hmem.
-    rewrite (Store.acc_upd_neq Hyx) (TypEnv.vsize_add_neq Hyx). exact: (Hcon _ Hmem).
-Qed.
+Module MakeBitsStore (V : SsrOrder) (TE : TypEnv with Module SE := V) <:
+  BitsStore V TE.
+
+  Include RealizableTStoreAdapter V BitsValueType.
+  Module Lemmas := FMapLemmas TE.
+
+  (* A store conforms to a typing environment if for every variable in the typing
+     environment, the size of its type in the typing environment is the same as
+     the size of its value in the store *)
+  Definition conform (s : t) (te : TE.env) : Prop :=
+    forall (v : V.t),
+      TE.mem v te -> TE.vsize v te = size (acc v s).
+
+  Lemma conform_mem v s te :
+    conform s te -> TE.mem v te -> TE.vsize v te = size (acc v s).
+  Proof. move=> H1 H2; exact: (H1 _ H2). Qed.
+
+  Lemma conform_upd x ty v s te :
+    sizeof_typ ty = size v ->
+    conform s te -> conform (upd x v s) (TE.add x ty te).
+  Proof.
+    move=> Hs Hcon y. case Hyx: (y == x).
+    - by rewrite (TE.vsize_add_eq Hyx) (acc_upd_eq Hyx).
+    - move/negP: Hyx => Hyx. rewrite (Lemmas.mem_add_neq Hyx) => Hmem.
+      move/negP: Hyx => Hyx. rewrite (acc_upd_neq Hyx) (TE.vsize_add_neq Hyx).
+      exact: (Hcon _ Hmem).
+  Qed.
+
+End MakeBitsStore.
+
+Module Store := MakeBitsStore VarOrder TE.
+Module SSAStore := MakeBitsStore SSAVarOrder SSATE.
+Module ZSSAStore := RealizableTStoreAdapter SSAVarOrder ZValueType.
+
+Section State.
+
+  Variable t : Type.
+
+  Inductive state : Type :=
+  | OK of t
+  | ERR.
+
+End State.
+
+Module State.
+  Definition t : Type := state Store.t.
+End State.
+
+Module SSAState.
+  Definition t : Type := state SSAStore.t.
+End SSAState.
+
+Module ZSSAState.
+  Definition t : Type := state ZSSAStore.t.
+End ZSSAState.
