src/BBAndSimple.v
@@ -2,7 +2,7 @@
 From Coq Require Import ZArith List.
 From mathcomp Require Import ssreflect ssrbool ssrnat eqtype seq tuple.
 From BitBlasting Require Import QFBVSimple CNFSimple BBCommonSimple.
-From ssrlib Require Import Var ZAriths Tuples Tactics.
+From ssrlib Require Import ZAriths Tuples Tactics.
 From Bits Require Import bits.
 
 Set Implicit Arguments.
